libcrux-ml-dsa/src/ml_dsa_generic/instantiations.rs
@@ -59,12 +59,32 @@ macro_rules! instantiate {
                             >(signing_key, message, context, randomness)
                         }
 
+                        /// Sign.
+                        pub fn sign_mut(
+                            signing_key: &[u8; SIGNING_KEY_SIZE],
+                            message: &[u8],
+                            context: &[u8],
+                            randomness: [u8; SIGNING_RANDOMNESS_SIZE],
+                            signature: &mut [u8; SIGNATURE_SIZE],
+                        ) -> Result<(), SigningError> {
+                            crate::ml_dsa_generic::$parameter_module::sign_mut::<
+                                $simdunit,
+                                $sampler,
+                                $shake128x4,
+                                $shake256,
+                                $shake256xof,
+                                $shake256x4,
+                            >(signing_key, message, context, randomness, signature)
+                        }
+
                         #[cfg(feature = "acvp")]
                         pub fn sign_internal(
                             signing_key: &[u8; SIGNING_KEY_SIZE],
                             message: &[u8],
                             randomness: [u8; SIGNING_RANDOMNESS_SIZE],
                         ) -> Result<MLDSASignature<SIGNATURE_SIZE>, SigningError> {
+                            let mut signature = MLDSASignature::zero();
+
                             crate::ml_dsa_generic::$parameter_module::sign_internal::<
                                 $simdunit,
                                 $sampler,
@@ -72,7 +92,9 @@ macro_rules! instantiate {
                                 $shake256,
                                 $shake256xof,
                                 $shake256x4,
-                            >(signing_key, message, None, randomness)
+                            >(signing_key, message, None, randomness, &mut signature.value)?;
+
+                            Ok(signature)
                         }
 
                         /// Sign (pre-hashed).
