libcrux-ml-dsa/proofs/fstar/extraction/Libcrux_ml_dsa.Ml_dsa_65_.Portable.fst
@@ -23,6 +23,21 @@ let generate_key_pair (randomness: t_Array u8 (sz 32)) =
   <:
   Libcrux_ml_dsa.Types.t_MLDSAKeyPair (sz 1952) (sz 4032)
 
+let generate_key_pair_mut
+      (randomness: t_Array u8 (sz 32))
+      (signing_key: t_Array u8 (sz 4032))
+      (verification_key: t_Array u8 (sz 1952))
+     =
+  let tmp0, tmp1:(t_Array u8 (sz 4032) & t_Array u8 (sz 1952)) =
+    Libcrux_ml_dsa.Ml_dsa_generic.Instantiations.Portable.Ml_dsa_65_.generate_key_pair randomness
+      signing_key
+      verification_key
+  in
+  let signing_key:t_Array u8 (sz 4032) = tmp0 in
+  let verification_key:t_Array u8 (sz 1952) = tmp1 in
+  let _:Prims.unit = () in
+  signing_key, verification_key <: (t_Array u8 (sz 4032) & t_Array u8 (sz 1952))
+
 let sign
       (signing_key: Libcrux_ml_dsa.Types.t_MLDSASigningKey (sz 4032))
       (message context: t_Slice u8)
@@ -36,6 +51,26 @@ let sign
     message
     context
     randomness
+
+let sign_mut
+      (signing_key: t_Array u8 (sz 4032))
+      (message context: t_Slice u8)
+      (randomness: t_Array u8 (sz 32))
+      (signature: t_Array u8 (sz 3309))
+     =
+  let tmp0, out:(t_Array u8 (sz 3309) &
+    Core.Result.t_Result Prims.unit Libcrux_ml_dsa.Types.t_SigningError) =
+    Libcrux_ml_dsa.Ml_dsa_generic.Instantiations.Portable.Ml_dsa_65_.sign_mut signing_key
+      message
+      context
+      randomness
+      signature
+  in
+  let signature:t_Array u8 (sz 3309) = tmp0 in
+  let hax_temp_output:Core.Result.t_Result Prims.unit Libcrux_ml_dsa.Types.t_SigningError = out in
+  signature, hax_temp_output
+  <:
+  (t_Array u8 (sz 3309) & Core.Result.t_Result Prims.unit Libcrux_ml_dsa.Types.t_SigningError)
 
 let sign_pre_hashed_shake128
       (signing_key: Libcrux_ml_dsa.Types.t_MLDSASigningKey (sz 4032))
