libcrux-ml-dsa/proofs/fstar/extraction/Libcrux_ml_dsa.Ml_dsa_generic.Instantiations.Avx2.Ml_dsa_65_.fst
@@ -64,6 +64,44 @@ let sign
       (randomness: t_Array u8 (sz 32))
      = sign___inner signing_key message context randomness
 
+let sign_mut___inner
+      (signing_key: t_Array u8 (sz 4032))
+      (message context: t_Slice u8)
+      (randomness: t_Array u8 (sz 32))
+      (signature: t_Array u8 (sz 3309))
+     =
+  let tmp0, out:(t_Array u8 (sz 3309) &
+    Core.Result.t_Result Prims.unit Libcrux_ml_dsa.Types.t_SigningError) =
+    Libcrux_ml_dsa.Ml_dsa_generic.Ml_dsa_65_.sign_mut #Libcrux_ml_dsa.Simd.Avx2.Vector_type.t_Vec256
+      #Libcrux_ml_dsa.Samplex4.Avx2.t_AVX2Sampler
+      #Libcrux_ml_dsa.Hash_functions.Simd256.t_Shake128x4
+      #Libcrux_ml_dsa.Hash_functions.Simd256.t_Shake256
+      #Libcrux_ml_dsa.Hash_functions.Portable.t_Shake256Xof
+      #Libcrux_ml_dsa.Hash_functions.Simd256.t_Shake256x4 (signing_key <: t_Slice u8) message
+      context randomness signature
+  in
+  let signature:t_Array u8 (sz 3309) = tmp0 in
+  let hax_temp_output:Core.Result.t_Result Prims.unit Libcrux_ml_dsa.Types.t_SigningError = out in
+  signature, hax_temp_output
+  <:
+  (t_Array u8 (sz 3309) & Core.Result.t_Result Prims.unit Libcrux_ml_dsa.Types.t_SigningError)
+
+let sign_mut
+      (signing_key: t_Array u8 (sz 4032))
+      (message context: t_Slice u8)
+      (randomness: t_Array u8 (sz 32))
+      (signature: t_Array u8 (sz 3309))
+     =
+  let tmp0, out:(t_Array u8 (sz 3309) &
+    Core.Result.t_Result Prims.unit Libcrux_ml_dsa.Types.t_SigningError) =
+    sign_mut___inner signing_key message context randomness signature
+  in
+  let signature:t_Array u8 (sz 3309) = tmp0 in
+  let hax_temp_output:Core.Result.t_Result Prims.unit Libcrux_ml_dsa.Types.t_SigningError = out in
+  signature, hax_temp_output
+  <:
+  (t_Array u8 (sz 3309) & Core.Result.t_Result Prims.unit Libcrux_ml_dsa.Types.t_SigningError)
+
 let sign_pre_hashed_shake128___inner
       (signing_key: t_Array u8 (sz 4032))
       (message context pre_hash_buffer: t_Slice u8)
